fstar/glue/proofs/MLS.NetworkBinder.Properties.fst
@@ -1,0 +1,19 @@
+module MLS.NetworkBinder.Properties
+
+open MLS.Tree
+open MLS.TreeCommon
+
+val path_filtering_ok:
+  #tree_leaf_t:Type -> #tree_node_t:Type ->
+  #path_leaf_t:Type -> #path_node_t:Type ->
+  #l:nat -> #i:tree_index l -> #li:leaf_index l i ->
+  tree (option tree_leaf_t) (option tree_node_t) l i -> path path_leaf_t (option path_node_t) l i li ->
+  prop
+let rec path_filtering_ok #tree_leaf_t #tree_node_t #path_leaf_t #path_node_t #l #i #li t p =
+  match t, p with
+  | TLeaf oln, PLeaf new_oln ->
+    True
+  | TNode _ _ _, PNode new_opn p_next ->
+    let (child, sibling) = get_child_sibling t li in
+    let node_ok = new_opn == None <==> is_tree_empty sibling in
+    node_ok /\ path_filtering_ok child p_next
