fstar/treekem/proofs/MLS.TreeKEM.Invariants.fst
@@ -1,0 +1,82 @@
+module MLS.TreeKEM.Invariants
+
+open Comparse
+open MLS.Crypto
+open MLS.Tree
+open MLS.TreeCommon
+open MLS.TreeKEM.Types
+
+val unmerged_leaf_exists:
+  #bytes:Type0 -> {|crypto_bytes bytes|} ->
+  #l:nat -> #i:tree_index l -> treekem bytes l i -> nat ->
+  prop
+let unmerged_leaf_exists #bytes #bl #l #i t li =
+  leaf_index_inside l i li && Some? (leaf_at t li)
+
+val treekem_invariant:
+  #bytes:Type0 -> {|crypto_bytes bytes|} ->
+  #l:nat -> #i:tree_index l ->
+  treekem bytes l i ->
+  prop
+let rec treekem_invariant #bytes #cb #l #i t =
+  match t with
+  | TLeaf oln ->
+    True
+  | TNode opn left right ->
+    let node_ok =
+      match opn with
+      | Some pn ->
+        Comparse.for_allP (unmerged_leaf_exists t) pn.unmerged_leaves
+      | None -> True
+    in
+    node_ok /\ treekem_invariant left /\ treekem_invariant right
+
+val treekem_priv_invariant:
+  #bytes:Type0 -> {|crypto_bytes bytes|} ->
+  #l:nat -> #i:tree_index l -> #li:leaf_index l i ->
+  treekem bytes l i -> treekem_priv bytes l i li ->
+  prop
+let rec treekem_priv_invariant #bytes #cb #l #i #li t p =
+  match t, p with
+  | TLeaf oln, PLeaf sk ->
+    //TODO: and oln contains sk's public key?
+    Some? oln
+  | TNode opn _ _, PNode osk p_next ->
+    let (child, _) = get_child_sibling t li in
+    treekem_priv_invariant child p_next
+
+val treekem_priv_invariant_leaf_at:
+  #bytes:Type0 -> {|crypto_bytes bytes|} ->
+  #l:nat -> #i:tree_index l -> #li:leaf_index l i ->
+  t:treekem bytes l i -> p:treekem_priv bytes l i li ->
+  Lemma
+  (requires treekem_priv_invariant t p)
+  (ensures Some? (leaf_at t li))
+let rec treekem_priv_invariant_leaf_at #bytes #cb #l #i #li t p =
+  match t, p with
+  | TLeaf oln, PLeaf sk -> ()
+  | TNode opn _ _, PNode osk p_next ->
+    let (child, _) = get_child_sibling t li in
+    treekem_priv_invariant_leaf_at child p_next
+
+/// Weaker variant of MLS.NetworkBinder.Properties.path_filtering_ok,
+/// where a sibling can be empty but the corresponding path node is non-empty.
+/// This is useful in TreeKEM,
+/// where there might be path secrets with empty siblings,
+/// because leaves added in the Commit are un-added before decrypting the path secret,
+/// hence when before the path is "filtering_ok",
+/// after un-adding the path becomes only "filtering_weak_ok".
+/// Fortunately, this is strong enough as a precondition to decrypt the path secret.
+val path_filtering_weak_ok:
+  #bytes:Type0 -> {|crypto_bytes bytes|} ->
+  #l:nat -> #i:tree_index l -> #li:leaf_index l i ->
+  treekem bytes l i -> pathkem bytes l i li ->
+  prop
+let rec path_filtering_weak_ok #bytes #bl #l #i #li t p =
+  match t, p with
+  | TLeaf oln, PLeaf new_oln ->
+    True
+  | TNode _ _ _, PNode new_opn p_next ->
+    let (child, sibling) = get_child_sibling t li in
+    let node_ok = new_opn == None ==> is_tree_empty sibling in
+    node_ok /\ path_filtering_weak_ok child p_next
